Protocol no longer TC, include protocol in all location assertions

src/high/protocol.v
@@ -11,35 +11,39 @@ From self.high.modalities Require Import no_buffer.
 Definition loc_pred `{nvmFixedG Σ} ST `{AbstractState ST} := ST → val → nvmDeltaG Σ → dProp Σ.
 
 (* A protocol consists of
-  - A predicate [ϕ] that holds for each write and corresponding state of the
+  - A predicate [pred] that holds for each write and corresponding state of the
     location.
   - A function [bumper] that specifies how the state of a location changes
     after a crash. *)
-Class LocationProtocol `{AbstractState ST, nvmFixedG Σ} (ϕ : loc_pred ST) := {
+Record LocationProtocol ST `{AbstractState ST, nvmFixedG Σ} := {
+  pred : loc_pred ST;
   bumper : ST → ST;
-  bumper_mono :> Proper ((⊑@{ST}) ==> (⊑))%signature bumper;
-  phi_condition :
+  bumper_mono : Proper ((⊑@{ST}) ==> (⊑))%signature bumper;
+  pred_condition :
     (⊢ ∀ (hD : nvmDeltaG Σ) s v,
-      ϕ s v hD -∗ <PCF> hD', ϕ (bumper s) v hD' : dProp Σ)%I;
-  phi_nobuf :> (∀ hD s v, IntoNoBuffer (ϕ s v hD) (ϕ s v hD));
+      pred s v hD -∗ <PCF> hD', pred (bumper s) v hD' : dProp Σ)%I;
+  pred_nobuf :> (∀ hD s v, IntoNoBuffer (pred s v hD) (pred s v hD));
 }.
 
-Global Arguments bumper {_} {_} {_} {_} {_} {_} _ {_} _.
+Global Arguments pred {ST} {_} {_} {_} {_} {_} _.
+Global Arguments bumper {ST} {_} {_} {_} {_} {_} _.
 
-Global Hint Mode LocationProtocol ! ! ! ! ! ! +  : typeclass_instances.
-(* Global Hint Mode LocationProtocol - - - - - - +  : typeclass_instances. *)
+Existing Instance bumper_mono.
+Existing Instance pred_nobuf.
 
 (** [know_protocol] represents the knowledge that a location is associated with a
 specific protocol. It's defined simply using more "primitive" assertions. *)
 Definition know_protocol `{AbstractState ST, nvmFixedG Σ, nvmDeltaG Σ}
-           ℓ (ϕ : loc_pred ST) `{!LocationProtocol ϕ} : dProp Σ :=
-  "#knowPred" ∷ ⎡ know_pred ℓ ϕ ⎤ ∗
-  "#knowPreorder" ∷ ⎡ know_preorder_loc ℓ (⊑@{ST}) ⎤ ∗
-  "#knowBumper" ∷ ⎡ know_bumper ℓ (bumper ϕ) ⎤%I.
+           ℓ (prot : LocationProtocol ST) : iProp Σ :=
+  "#knowPred" ∷ know_pred ℓ prot.(pred) ∗
+  "#knowPreorder" ∷ know_preorder_loc ℓ (⊑@{ST}) ∗
+  "#knowBumper" ∷ know_bumper ℓ prot.(bumper).
 
-Lemma encode_bumper_bump_mono `{LocationProtocol ST} (x y x' y' : positive) :
-  encode_bumper (bumper ϕ) x = Some x' →
-  encode_bumper (bumper ϕ) y = Some y' →
+Lemma encode_bumper_bump_mono `{AbstractState ST}
+      (bumper : ST → ST) `{!Proper ((⊑@{ST}) ==> (⊑))%signature bumper}
+      (x y x' y' : positive) :
+  encode_bumper bumper x = Some x' →
+  encode_bumper bumper y = Some y' →
   encode_relation (⊑@{ST}) x y →
   encode_relation (⊑@{ST}) x' y'.
 Proof.
@@ -53,20 +57,22 @@ Qed.
 Section protocol.
   Context `{nvmFixedG Σ, nvmDeltaG Σ, AbstractState ST}.
 
-  Implicit Types (ϕ : loc_pred ST).
+  Implicit Types (prot : LocationProtocol ST).
 
-  Lemma post_crash_know_protocol ℓ ϕ `{!LocationProtocol ϕ} :
-    know_protocol ℓ ϕ -∗ <PC> hD, or_lost ℓ (know_protocol ℓ ϕ).
+  Lemma post_crash_know_protocol ℓ prot :
+    ⎡ know_protocol ℓ prot ⎤ -∗ <PC> hD, or_lost ℓ (⎡ know_protocol ℓ prot ⎤).
   Proof.
-    iIntros "(? & ? & ?)". iCrash.
-    rewrite /know_protocol. rewrite -?or_lost_sep.
-    iFrame.
+    iIntros "(a & b & c)". iCrash.
+    iCombine "a b c" as "a".
+    rewrite ?or_lost_sep.
+    iApply (or_lost_mono with "[] a").
+    iIntros "($ & $ & $)".
   Qed.
 
-  Global Instance know_protocol_into_crash ℓ ϕ `{!LocationProtocol ϕ} :
+  Global Instance know_protocol_into_crash ℓ prot :
     IntoCrash
-      (know_protocol ℓ ϕ)%I
-      (λ hG', or_lost ℓ (know_protocol ℓ ϕ))%I.
+      (⎡ know_protocol ℓ prot ⎤)%I
+      (λ hG', or_lost ℓ (⎡ know_protocol ℓ prot ⎤))%I.
   Proof.
     rewrite /IntoCrash. iIntros "P". by iApply post_crash_know_protocol.
   Qed.
